src/Narcissus/Formats/SizedListOpt.v
@@ -4,6 +4,7 @@ Require Import
 
 Require Import
         Fiat.CommonEx
+        Fiat.Narcissus.BinLib.Core
         Fiat.Narcissus.Common.Notations
         Fiat.Narcissus.Common.Specs
         Fiat.Narcissus.Common.ComposeOpt.
@@ -25,6 +26,11 @@ Section SizedList.
   Variable A_format_byte : forall d b ce ce', A_format d ce ↝ (b, ce') -> bin_measure b mod 8 = 0.
   Variable A_decode_lt : forall b cd x b' cd', A_decode b cd = Some (x, b', cd') -> lt_B b' b.
   Variable A_decode_correct : CorrectDecoder monoid A_predicate A_predicate_rest A_format A_decode A_cache_inv.
+
+  Variable Wf_bound : B.
+  Variable Wf_decode : forall b, lt_B b Wf_bound -> CacheDecode -> option (A * B * CacheDecode).
+  Variable Wf_decode_lt : forall b pf cd x b' cd', Wf_decode b pf cd = Some (x, b', cd') -> lt_B b' b.
+  Variable Wf_decode_correct : CorrectDecoderWf monoid A_predicate A_predicate_rest A_format Wf_decode A_cache_inv.
 
   Definition SizedList_format : FormatM (list A) B :=
     fix format xs ce :=
@@ -51,7 +57,72 @@ Section SizedList.
                   `(xs, b2, cd2) <- decode (sz - (bin_measure b - bin_measure (proj1_sig b1))) _ (proj1_sig b1) cd1;
                 Some (x :: xs, b2, cd2)
               end)).
-    destruct b1. unfold lt_B in *. simpl in *. abstract omega.
+    abstract (destruct b1; unfold lt_B in *; simpl in *; omega).
+  Defined.
+
+  Definition Decode_w_Measure_lt_wf
+             (b : B)
+             (pf : lt_B b Wf_bound)
+             (cd : CacheDecode)
+    : option (A * {b' : B | lt_B b' b} * CacheDecode).
+    generalize (Wf_decode_lt b pf cd); clear.
+    destruct (Wf_decode b pf cd) as [ [ [ a b' ] cd' ] | ]; intros;
+      [ refine (Some (a, exist _ b' (H _ _ _ eq_refl), cd'))
+      | exact None ].
+  Defined.
+
+  Lemma Decode_w_Measure_lt_eq_wf
+        (b : B)
+        (pf : lt_B b Wf_bound)
+        (cd : CacheDecode)
+    : forall a' b' cd',
+      Wf_decode b pf cd = Some (a', b', cd')
+      -> exists pf',
+        Decode_w_Measure_lt_wf b pf cd =
+        Some (a', exist _ b' pf', cd').
+  Proof.
+    clear; intros; unfold Decode_w_Measure_lt_wf.
+    remember (Wf_decode_lt b pf cd); clear Heql.
+    destruct (Wf_decode b pf cd) as [ [ [? ?] ? ] | ].
+    injections; eauto.
+    discriminate.
+  Qed.
+
+  Lemma Decode_w_Measure_lt_eq_inv_wf
+        (b : B)
+        (pf : lt_B b Wf_bound)
+        (cd : CacheDecode)
+    : forall (a' : A) (cd' : CacheDecode)
+        pf',
+      Decode_w_Measure_lt_wf b pf cd = Some (a', pf', cd')
+      -> Wf_decode b pf cd = Some (a', `pf' , cd').
+  Proof.
+    unfold Decode_w_Measure_lt_wf; intros.
+    revert pf' H.
+    generalize (Wf_decode_lt b pf cd).
+    destruct (Wf_decode b pf cd) as [ [ [? ?] ?] | ]; simpl; intros;
+      try discriminate.
+    injections; reflexivity.
+  Qed.
+
+  Definition SizedListWf_decode : nat -> forall b, lt_B b Wf_bound -> CacheDecode -> option (list A * B * CacheDecode).
+  Proof.
+    refine
+      (Fix lt_wf _
+           (fun sz decode b pf cd =>
+              match sz with
+              | O => Some (nil, b, cd)
+              | _ =>
+                `(x, b1, cd1) <- Decode_w_Measure_lt_wf b _ cd;
+                if lt_dec sz (bin_measure b - bin_measure (proj1_sig b1)) then
+                  None
+                else
+                  `(xs, b2, cd2) <- decode (sz - (bin_measure b - bin_measure (proj1_sig b1))) _ (proj1_sig b1) _ cd1;
+                Some (x :: xs, b2, cd2)
+              end)).
+    abstract assumption.
+    abstract (destruct b1; unfold lt_B in *; simpl in *; omega).
+    abstract (destruct b1; unfold lt_B in *; simpl in *; omega).
   Defined.
 
   Theorem SizedList_decode_le
@@ -59,6 +130,22 @@ Section SizedList.
       SizedList_decode sz b cd = Some (xs, b', cd') -> le_B b' b.
   Proof.
     unfold SizedList_decode.
+    induction sz using (well_founded_ind lt_wf); intros.
+    rewrite Coq.Init.Wf.Fix_eq in H0 by solve_extensionality.
+    destruct sz. injections. unfold le_B. easy.
+    decode_opt_to_inv. destruct lt_dec. easy.
+    decode_opt_to_inv. subst. destruct x0.
+    remember (S sz) as sz'.
+    unfold lt_B, le_B in *.
+    apply H in H1; clear H;
+      simpl in *; omega.
+  Qed.
+
+  Theorem SizedListWf_decode_le
+    : forall sz b pf cd xs b' cd',
+      SizedListWf_decode sz b pf cd = Some (xs, b', cd') -> le_B b' b.
+  Proof.
+    unfold SizedListWf_decode.
     induction sz using (well_founded_ind lt_wf); intros.
     rewrite Coq.Init.Wf.Fix_eq in H0 by solve_extensionality.
     destruct sz. injections. unfold le_B. easy.
@@ -199,6 +286,125 @@ Section SizedList.
         - simpl. rewrite <- mappend_assoc. subst. auto.
         - intros. computes_to_inv2.
           specialize (H11 _ _ _ H14'). rewrite !mappend_measure in *.
+          assert (bin_measure b1 = bin_measure x2). {
+            eapply A_format_sz_eq; eauto.
+          } omega.
+        - destruct 1; subst; auto.
+        - auto.
+      }
+    }
+  Qed.
+
+  Theorem SizedListWf_decode_correct
+    : forall sz,
+      CorrectDecoderWf
+        monoid
+        (fun xs =>
+           (forall b ce ce', SizedList_format xs ce ↝ (b, ce') -> bin_measure b = sz) /\
+           forall x, In x xs -> A_predicate x)
+        SizedList_predicate_rest
+        SizedList_format (SizedListWf_decode sz) A_cache_inv.
+  Proof.
+    unfold SizedList_format, SizedListWf_decode.
+    split; intros. {
+      generalize dependent sz.
+      generalize dependent env.
+      generalize dependent env'.
+      generalize dependent xenv.
+      generalize dependent ext.
+      generalize dependent bin.
+      induction data; intros. {
+        eexists.
+        destruct H0 as [H3 H4]. specialize (H3 _ _ _ H2).
+        inversion H2. clear H2. subst.
+        repeat split; eauto.
+        rewrite Coq.Init.Wf.Fix_eq by solve_extensionality.
+        rewrite mempty_measure_0.
+        repeat progress f_equal. rewrite mempty_left. auto.
+      } {
+        destruct H0 as [H3 H4]. specialize (H3 _ _ _ H2).
+        computes_to_inv2. revert pf. rewrite <- mappend_assoc. intros.
+        assert (lt_B (mappend b ext) Wf_bound) as pf'. {
+          unfold lt_B in *. rewrite !mappend_measure in pf. rewrite mappend_measure. omega.
+        }
+        destruct Wf_decode_correct as [He _].
+        simpl in H1. destruct H1. specialize (H0 _ _ _ H2').
+        edestruct He with (ext:=mappend b ext) (pf := pf); eauto.
+        apply H4. intuition. destruct_many.
+        rewrite mappend_measure.
+        edestruct IHdata with (ext:=ext) (pf:=pf'); intros; eauto.
+        split. intros. eapply SizedList_format_sz_eq; eauto.
+        intros. apply H4. intuition. clear IHdata.
+        eexists; intuition; eauto.
+        rewrite Coq.Init.Wf.Fix_eq by solve_extensionality; simpl.
+        match goal with
+        | _ : _ |- context [match ?a with _ => _ end] => destruct a eqn:?
+        end.
+        apply Wf_decode_lt in H3.
+        unfold lt_B in *.
+        repeat match goal with
+               | H : context [bin_measure (mappend _ _)] |- _ => rewrite !mappend_measure in H
+               end; omega.
+        edestruct @Decode_w_Measure_lt_eq_wf; eauto.
+        simpl in *.
+        match goal with
+        | |- context [Decode_w_Measure_lt_wf _ ?a _] => replace a with pf in * by apply le_uniqueness_proof
+        end. rewrite H9. simpl. clear H9. destruct lt_dec.
+        repeat match goal with
+               | H : context [bin_measure (mappend _ _)] |- _ => rewrite !mappend_measure in H
+               end; omega.
+        match goal with
+        | _ : _ |- context [Fix _ _ _ ?a _ _ _] =>
+          replace a with (bin_measure b)
+        end. simpl in H8.
+        match goal with
+        | H : context [Fix _ _ _ _ _ ?p _]
+          |- context [Fix _ _ _ _ _ ?p' _] =>
+          replace p' with p by apply le_uniqueness_proof
+        end.
+        rewrite H8. auto.
+        unfold lt_B in *. rewrite !mappend_measure in *.
+        match goal with
+        | _ : _ |- context [match ?a with _ => _ end] =>
+          replace a with (bin_measure b0) by omega
+        end.
+        destruct (bin_measure b0) eqn:Heq; simpl in *; omega.
+      }
+    } {
+      generalize dependent env.
+      generalize dependent env'.
+      generalize dependent xenv'.
+      generalize dependent data.
+      generalize dependent ext.
+      generalize dependent bin.
+      induction sz using (well_founded_ind lt_wf); intros.
+      rewrite Coq.Init.Wf.Fix_eq in H1 by solve_extensionality.
+      destruct sz. {
+        inversion H1. clear H1. subst. split; auto.
+        exists mempty, env. repeat split; intros; auto.
+        - symmetry. apply mempty_left.
+        - inversion H1. apply mempty_measure_0.
+        - inversion H1.
+      } {
+        decode_opt_to_inv.
+        destruct x0. simpl proj1_sig in H3. simpl proj2_sig in H3.
+        apply Decode_w_Measure_lt_eq_inv_wf in H1. simpl in H1.
+        destruct Wf_decode_correct as [_ Hd]; auto.
+        edestruct Hd; eauto. clear Hd. destruct_many.
+        destruct lt_dec; try congruence.
+        decode_opt_to_inv. subst.
+        edestruct H; try apply H3; eauto. unfold lt_B in l. omega.
+        destruct_many.
+        split; eauto. eexists _, _. repeat split.
+        - computes_to_econstructor; eauto.
+          computes_to_econstructor; eauto.
+        - simpl. rewrite <- mappend_assoc. subst. auto.
+        - intros. computes_to_inv2.
+          specialize (H11 _ _ _ H14').
+          clear H3.
+          repeat match goal with
+                 | H : context [bin_measure (mappend _ _)] |- _ => rewrite !mappend_measure in H
+                 end. rewrite !mappend_measure.
           assert (bin_measure b1 = bin_measure x2). {
             eapply A_format_sz_eq; eauto.
           } omega.
